## Question 1

> Questions below are related to the following table. Let $A, B, C \in \{0,1\}$ be three binary random variables with the following joint probability distribution:


| a  | b  | c  | f(a,b,c) |
|----|----|----|----------|
| 0  | 0  | 0  | 0.01     |
| 0  | 0  | 1  | 0.07     |
| 0  | 1  | 0  | 0.02     |
| 0  | 1  | 1  | 0.10     |
| 1  | 0  | 0  | 0.02     |
| 1  | 0  | 1  | 0.30     |
| 1  | 1  | 0  | 0.04     |
| 1  | 1  | 1  | 0.44     |


> By direct calculation, compute the marginal $P(A,B)$.
> 
> (Recall that $P(A,B)$ is represented by 4 numbers: $P(A = 0, B = 0)$, $P(A = 0, B = 1)$, $P(A = 1, B = 0)$, $P(A = 1, B = 1)$.)

-------

The marginal pmf of two discrete random variables $A$ and $B$ is the sum of the joint pmf $f(A, B, C)$ over all possible values of $C$ for each combination of $A$ and $B$. This is given by:

$$
f_{A,B}(a, b) = \sum_{\forall c} f(a, b, c)
$$

Since the table provides the probability of each joint event of $A$, $B$, and $C$, we can directly calculate the marginal pmf of $A$ and $B$ by summing the joint pmf over all values of $C$.

### Calculation of $P(A, B)$:

For $A = 0, B = 0$:

$$
f_{A,B}(0, 0) = f(0, 0, 0) + f(0, 0, 1) = 0.01 + 0.07 = 0.08
$$

For $A = 0, B = 1$:

$$
f_{A,B}(0, 1) = f(0, 1, 0) + f(0, 1, 1) = 0.02 + 0.10 = 0.12
$$

For $A = 1, B = 0$:

$$
f_{A,B}(1, 0) = f(1, 0, 0) + f(1, 0, 1) = 0.02 + 0.30 = 0.32
$$

For $A = 1, B = 1$:

$$
f_{A,B}(1, 1) = f(1, 1, 0) + f(1, 1, 1) = 0.04 + 0.44 = 0.48
$$

### Conclusion:

Therefore, the marginal pmf of $A$ and $B$ is:

$$
f_{A,B}(a, b) =
\begin{cases}
0.08 & \text{if } a = 0, b = 0 \\
0.12 & \text{if } a = 0, b = 1 \\
0.32 & \text{if } a = 1, b = 0 \\
0.48 & \text{if } a = 1, b = 1
\end{cases}
$$


## Question 2

> By direct calculation compute the marginals $P(A)$ and $P(B)$.

-------

To find the marginal pmf of $A$, we sum the joint pmf $f(A, B, C)$ over all possible values of $B$ and $C$ for each value of $A$. Similarly, to find the marginal pmf of $B$, we sum the joint pmf $f(A, B, C)$ over all possible values of $A$ and $C$ for each value of $B$.

### Calculation of $P(A)$:

For $A = 0$:

$$
f_A(0) = f(0, 0, 0) + f(0, 0, 1) + f(0, 1, 0) + f(0, 1, 1) = 0.01 + 0.07 + 0.02 + 0.10 = 0.20
$$

For $A = 1$:

$$
f_A(1) = f(1, 0, 0) + f(1, 0, 1) + f(1, 1, 0) + f(1, 1, 1) = 0.02 + 0.30 + 0.04 + 0.44 = 0.80
$$

### Calculation of $P(B)$:

For $B = 0$:

$$
f_B(0) = f(0, 0, 0) + f(1, 0, 0) + f(1, 0, 1) + f(0, 0, 1) = 0.01 + 0.02 + 0.30 + 0.07 = 0.40
$$

For $B = 1$:

$$
f_B(1) = f(0, 1, 0) + f(1, 1, 0) + f(1, 1, 1) + f(0, 1, 1) = 0.02 + 0.04 + 0.44 + 0.10 = 0.60
$$

### Conclusion:

Therefore, the marginal pmf of $A$ and $B$ is:

$$
f_A(a) =
\begin{cases}
0.20 & \text{if } a = 0 \\
0.80 & \text{if } a = 1
\end{cases}
$$

$$
f_B(b) =
\begin{cases}
0.40 & \text{if } b = 0 \\
0.60 & \text{if } b = 1
\end{cases}
$$


## Question 3

> Are the random variables $A$ and $B$ independent? Why or why not?

----

Two random variables $A$ and $B$ are independent if and only if their joint pmf is the product of their marginal pmfs for all possible values of $A$ and $B$. In other words, $A$ and $B$ are independent if:

$$
f_{A, B}(a, b) = f_A(a) \cdot f_B(b)
$$

for all possible values of $A$ and $B$. This definition implies that the occurrence of one event does not affect the occurrence of the other event.

To check if $A$ and $B$ are independent, we compare the joint pmf $f_{A, B}(a, b)$ with the product of the marginal pmfs $f_A(a) \cdot f_B(b)$ for all possible values of $A$ and $B$:

For $A = 0, B = 0$:

$$
f_{A, B}(0, 0) = 0.08 = 0.20 \cdot 0.40 = 0.08
$$

For $A = 0, B = 1$:

$$
f_{A, B}(0, 1) = 0.12 = 0.20 \cdot 0.60 = 0.12
$$

For $A = 1, B = 0$:

$$
f_{A, B}(1, 0) = 0.32 = 0.80 \cdot 0.40 = 0.32
$$

For $A = 1, B = 1$:

$$
f_{A, B}(1, 1) = 0.48 = 0.80 \cdot 0.60 = 0.48
$$

Since for all possible values of $A$ and $B$, $f_{A, B}(a, b) = f_A(a) \cdot f_B(b)$, the random variables $A$ and $B$ are **independent**.

## Question 4

> Compute the conditional distribution $P(A, B | C)$. 
> 
> Note that this includes computing $P(A, B | C = 0)$ as well as $P(A, B | C = 1)$, each of which is represented by 4 numbers (in total 8 numbers).

A conditional probability for two random variables $X$ and $Y$ is given by:

$$
P(X | Y) = \frac{P(X, Y)}{P(Y)}
$$

where $P(X, Y)$ is the joint probability of $X$ and $Y$, and $P(Y)$ is the marginal probability of $Y$.

Extending this to three random variables $A$, $B$, and $C$, the conditional probability $P(A, B | C)$ is given by:

$$
P(A, B | C = c) = \frac{P(A, B, C = c)}{P(C = c)}
$$

where $P(A, B, C)$ is the joint probability of $A$, $B$, and $C$, and $P(C)$ is the marginal probability of $C$.

#### Calculate the marginal probability of $C$

For $C = 0$:

$$
f_C(0) = f(0, 0, 0) + f(1, 0, 0) + f(1, 1, 0) + f(0, 1, 0) = 0.01 + 0.02 + 0.04 + 0.02 = 0.09
$$

Since $C$ is a binary random variable, $P(C = 1) = 1 - P(C = 0) = 1 - 0.09 = 0.91$.

#### Calculate the conditional probability of $A, B | C$

For $A = 0, B = 0, C = 0$:

$$
f(0, 0, 0) = 0.01 \implies f(0, 0 | 0) = \frac{f(0, 0, 0)}{f_C(0)} = \frac{0.01}{0.09} = 0.1111
$$

For $A = 0, B = 0, C = 1$:

$$
f(0, 0, 1) = 0.07 \implies f(0, 0 | 1) = \frac{f(0, 0, 1)}{f_C(1)} = \frac{0.07}{0.91} = 0.0769
$$

For $A = 0, B = 1, C = 0$:

$$
f(0, 1, 0) = 0.02 \implies f(0, 1 | 0) = \frac{f(0, 1, 0)}{f_C(0)} = \frac{0.02}{0.09} = 0.2222
$$

For $A = 0, B = 1, C = 1$:

$$
f(0, 1, 1) = 0.10 \implies f(0, 1 | 1) = \frac{f(0, 1, 1)}{f_C(1)} = \frac{0.10}{0.91} = 0.1099
$$

For $A = 1, B = 0, C = 0$:

$$
f(1, 0, 0) = 0.02 \implies f(1, 0 | 0) = \frac{f(1, 0, 0)}{f_C(0)} = \frac{0.02}{0.09} = 0.2222
$$

For $A = 1, B = 0, C = 1$:

$$
f(1, 0, 1) = 0.30 \implies f(1, 0 | 1) = \frac{f(1, 0, 1)}{f_C(1)} = \frac{0.30}{0.91} = 0.3297
$$

For $A = 1, B = 1, C = 0$:

$$
f(1, 1, 0) = 0.04 \implies f(1, 1 | 0) = \frac{f(1, 1, 0)}{f_C(0)} = \frac{0.04}{0.09} = 0.4444
$$

For $A = 1, B = 1, C = 1$:

$$
f(1, 1, 1) = 0.44 \implies f(1, 1 | 1) = \frac{f(1, 1, 1)}{f_C(1)} = \frac{0.44}{0.91} = 0.4835
$$

### Conclusion:

Therefore, the conditional pmf of $A$ and $B$ given $C$ is:

$$
f_{A,B|C}(a, b | c) =
\begin{cases}
0.1111 & \text{if } a = 0, b = 0, c = 0 \\
0.0769 & \text{if } a = 0, b = 0, c = 1 \\
0.2222 & \text{if } a = 0, b = 1, c = 0 \\
0.1099 & \text{if } a = 0, b = 1, c = 1 \\
0.2222 & \text{if } a = 1, b = 0, c = 0 \\
0.3297 & \text{if } a = 1, b = 0, c = 1 \\
0.4444 & \text{if } a = 1, b = 1, c = 0 \\
0.4835 & \text{if } a = 1, b = 1, c = 1
\end{cases}
$$




## Question 5

> Let
>
> $$
> f(x, y) = 
> \begin{cases}
> c(x + y^2) & \text{for } 0 \leq x \leq 1, 0 \leq y \leq 1 \\
> 0 & \text{otherwise}
> \end{cases}
> $$
>
>
> Find $P(X \leq \frac{1}{2} | Y = \frac{1}{2})$.

-----

For a continuous random variable, the probability of an event is given by the integral of the joint PDF over the region corresponding to the event. In this case, we need to find the probability that $X$ is less than or equal to $\frac{1}{2}$ given that $Y = \frac{1}{2}$.

From the definition of conditional probability for continuous random variables, we have:

$$
P(X \leq \frac{1}{2} \mid Y = \frac{1}{2}) = \frac{P(X \leq \frac{1}{2}, Y = \frac{1}{2})}{P(Y = \frac{1}{2})}
$$

where $P(X \leq \frac{1}{2}, Y = \frac{1}{2})$ is the joint PDF of $X$ and $Y$, and $P(Y = \frac{1}{2})$ is the marginal PDF of $Y$ at $y = \frac{1}{2}$.

### Calculate the marginal PDF of $Y$

The marginal PDF of $Y$ is obtained by integrating the joint PDF over all possible values of $X$ (in this case, from 0 to 1):

$$
f_Y(y) = \int_{0}^{1} c(x + y^2) dx = c \left[ \frac{x^2}{2} + y^2x \right]_{0}^{1} = c \left( \frac{1}{2} + y^2 \right)
$$

For $Y = \frac{1}{2}$:

$$
f_Y\left(\frac{1}{2}\right) = c \left( \frac{1}{2} + \left(\frac{1}{2}\right)^2 \right) = c \left( \frac{1}{2} + \frac{1}{4} \right) = c \left( \frac{3}{4} \right)
$$

### Calculate $P(X \leq \frac{1}{2}, Y = \frac{1}{2})$

Next, calculate the joint probability $P(X \leq \frac{1}{2}, Y = \frac{1}{2})$ by integrating the joint PDF over the region defined by $0 \leq x \leq \frac{1}{2}$ and $y = \frac{1}{2}$:

$$
P(X \leq \frac{1}{2}, Y = \frac{1}{2}) = \int_{0}^{\frac{1}{2}} c(x + \left(\frac{1}{2}\right)^2) dx = c \left[ \frac{x^2}{2} + \frac{1}{4}x \right]_{0}^{\frac{1}{2}} = c \left( \frac{1}{8} + \frac{1}{8} \right) = c \left( \frac{1}{4} \right)
$$

### Calculate the conditional probability

Now we can calculate the conditional probability:

$$
P(X \leq \frac{1}{2} \mid Y = \frac{1}{2}) = \frac{P(X \leq \frac{1}{2}, Y = \frac{1}{2})}{P(Y = \frac{1}{2})} = \frac{c \left( \frac{1}{4} \right)}{c \left( \frac{3}{4} \right)} = \frac{\frac{1}{4}}{\frac{3}{4}} = \frac{1}{3}
$$

### Conclusion:

The conditional probability is:

$$
P(X \leq \frac{1}{2} \mid Y = \frac{1}{2}) = \frac{1}{3}
$$

## Question 6


> Assume there are 100 boys and 150 girls in a classroom. We are going to select 70 students at random from the classroom without replacement. Let X denote the number of boys that are selected and let Y denote the number of girls that are selected. Find the expectation of X −Y .

---

From the properties of expectation, we know that the expectation of the difference of two random variables is the difference of their expectations. Therefore, we can find the expectation of $X - Y$ by finding the expectations of $X$ and $Y$ separately and then taking their difference.

Since we are sampling without replacement, we know to use the hypergeometric distribution given by:

$$
P(X = x) = \frac{{A \choose x} {B \choose n-x}}{{A+B \choose n}}
$$

In this case:

- $A = 100$
- $B = 150$
- $n = 70$

### Calculate the expectation of $X$

The expectation of a hypergeometric distribution is given by:

$$
E(X) = \sum_{x=0}^{n} x \cdot P(X = x)
$$

Substitute the values into the formula:

$$
E(X) = \sum_{x=0}^{70} x \cdot \frac{{100 \choose x} {150 \choose 70-x}}{{250 \choose 70}} = 28
$$

### Calculate the expectation of $Y$

Similarly, the expectation of $Y$ is:

$$
E(Y) = \sum_{y=0}^{70} y \cdot \frac{{150 \choose y} {100 \choose 70-y}}{{250 \choose 70}} = 42
$$

### Calculate the expectation of $X - Y$

Finally, the expectation of $X - Y$ is the difference of the expectations of $X$ and $Y$:

$$
E(X - Y) = E(X) - E(Y) = 28 - 42 = -14
$$

## Question 7

> Assume $X$, $Y$ are two random variables that have a negative correlation. Determine the relationship between $Var(X + Y )$ and $Var(X - Y)$ (i.e. find out whether the former is larger or smaller than the latter).

----

Variance of $X + Y$ is given by:

$$
Var(X + Y) = E[(X + Y)^2] - E[X + Y]^2 = Var(X) + Var(Y) + 2Cov(X, Y)
$$

Variance of $X - Y$ is given by:

$$
Var(X - Y) = E[(X - Y)^2] - E[X - Y]^2 = Var(X) + Var(Y) - 2Cov(X, Y)
$$

Covariance is a measure of the relationship between two random variables. If two random variables have a negative correlation, it means that as one variable increases, the other variable decreases. It is given by:

$$
Cov(X, Y) = E[XY] - E[X]E[Y] = \sigma_X \sigma_Y \rho_{X, Y}
$$


The correlation of $X$ and $Y$ is given by:

$$
\rho_{X, Y} = \frac{Cov(X, Y)}{\sqrt{Var(X)Var(Y)}} = \frac{Cov(X, Y)}{\sigma_X \sigma_Y}
$$

Since the product of the sigmas cannot be negative, if the correlation is negative $\implies$ the covariance is negative:

$$
Cov(X, Y) < 0
$$

Since $Var(X + Y) = Var(X) + Var(Y) + 2Cov(X, Y)$ and $Var(X - Y) = Var(X) + Var(Y) - 2Cov(X, Y)$, when $Cov(X, Y) < 0$, the variance of $X - Y$ will increase by $2 \cdot |Cov(X, Y)|$ whereas the variance of $X + Y$ reduces by $2 \cdot |Cov(X, Y)|$ compared to the variance of $X$ and $Y$.

Thus, the relationship between $Var(X + Y)$ and $Var(X - Y)$ is:

$$
\rho_{X, Y} < 0 \implies Cov(X, Y) < 0 \implies Var(X - Y) > Var(X + Y)
$$

## Question 8

> Questions below are related to random variable X ∼N(3,16). You need to use scipy.stats. Paste your relevant code for each question separately.


